Allow for some objects to not be virtually destroyed.
Virtual dispatch to destrutors only occurs on [delete].

theories/lang/cpp/logic/destroy.v
@@ -1,9 +1,10 @@
 (*
- * Copyright (c) 2020 BedRock Systems, Inc.
+ * Copyright (c) 2020-2021 BedRock Systems, Inc.
  * This software is distributed under the terms of the BedRock Open-Source License.
  * See the LICENSE-BedRock file in the repository root for details.
  *)
 Require Import Coq.ZArith.ZArith.
+Require Import iris.proofmode.tactics.
 Require Import bedrock.lang.cpp.ast.
 Require Import bedrock.lang.cpp.semantics.
 From bedrock.lang.cpp.logic Require Import
@@ -20,58 +21,97 @@ Section destroy.
   Local Notation anyR := (anyR (resolve:=σ)) (only parsing).
   Local Notation _global := (_global (resolve:=σ)) (only parsing).
 
-  (* this destructs an object by invoking its destructor
-     note: it does *not* free the underlying memory.
+  (** [resolve_dtor cls this Q] reduces to [Q dtor' this'] where [dtor'] is the
+      destructor to be called on [this'] which is used to destroy [this].
    *)
-  Definition destruct_obj (dtor : obj_name) (cls : globname) (v : ptr) (Q : mpred) : mpred :=
+  Definition resolve_dtor (cls : globname) (this : ptr) (Q : forall (faddr : ptr) (cls_name : globname) (this_addr : ptr), mpred)
+    : mpred :=
     match σ.(genv_tu) !! cls with
     | Some (Gstruct s) =>
-      match σ.(genv_tu) !! dtor with
-      | Some ov =>
-        let ty := type_of_value ov in
-        let dtor := s.(s_dtor) in
-        if has_virtual_dtor s then
-          resolve_virtual (σ:=σ) v cls dtor (fun da p =>
-             |> mspec σ.(genv_tu).(globals) (Tnamed cls) ty ti (Vptr da) (Vptr p :: nil) (fun _ => Q))
-        else
-             |> mspec σ.(genv_tu).(globals) (Tnamed cls) ty ti (Vptr $ _global dtor) (Vptr v :: nil) (fun _ => Q)
-      | _ => False
-      end
+      if has_virtual_dtor s then
+        resolve_virtual this cls s.(s_dtor) Q
+      else
+        Q (_global s.(s_dtor)) cls this
+    | Some (Gunion u) => Q (_global u.(u_dtor)) cls this
     | _ => False
-    end.
+    end%I.
 
-  (* [destruct_val t this dtor Q] invokes the destructor ([dtor]) on [this]
+  Lemma resolve_dtor_frame : forall cls this Q Q',
+      Forall a b c, Q a b c -* Q' a b c |-- resolve_dtor cls this Q -* resolve_dtor cls this Q'.
+  Proof.
+    rewrite /resolve_dtor.
+    intros. case_match; eauto.
+    case_match; eauto.
+    { iIntros "X"; iApply "X". }
+    { case_match.
+      { iApply resolve_virtual_frame. }
+      { iIntros "X"; iApply "X". } }
+  Qed.
+
+  (* [destruct_val dispatch t this dtor Q] invokes the destructor ([dtor]) on [this]
      with the type of [this] is [t].
+
+     The [dispatch] parameter determines whether the call is a *potentially* virtual call.
+     If [dispatch] is true *and the destructor of the class is virtual, then the call is a
+     virtual call.
 
      note: it does *not* free the underlying memory.
 
-     NOTE since we switched to using implicit destructors, we no longer need to worry about
-          invoking the destructor if [dtor] is [None].
+     TODO we can remove [dtor] with the new desructor scheme
    *)
-  Fixpoint destruct_val (t : type) (this : ptr) (dtor : option obj_name) (Q : mpred)
+  Fixpoint destruct_val (dispatch : bool) (t : type) (this : ptr) (dtor : option obj_name) (Q : mpred)
            {struct t}
   : mpred :=
     match t with
-    | Tqualified _ t => destruct_val t this dtor Q
+    | Tqualified _ t => destruct_val dispatch t this dtor Q
     | Tnamed cls =>
-      let continue dtor := destruct_obj dtor cls this Q in
-      match dtor with
-      | None =>
-        |={↑pred_ns}=> this |-> tblockR t 1 ** (this |-> tblockR t 1 -* Q)
-(*        match σ.(genv_tu) !! cls with
-               | Some (Gstruct s) => continue s.(s_dtor)
-               | Some (Gunion u) => continue u.(u_dtor)
-               | _ => False
-               end
-*)
-      | Some dtor => continue dtor
-      end
+      if dispatch then
+        resolve_dtor cls this (fun fimpl impl_class this' =>
+          let ty := Tmember_func (Tnamed impl_class) $ Tfunction Tvoid nil in
+          |> mspec σ.(genv_tu).(globals) (Tnamed cls) ty ti (Vptr fimpl) (Vptr this' :: nil) (fun _ => Q))
+      else
+        let continue dtor :=
+          let ty := Tmember_func (Tnamed cls) $ Tfunction Tvoid nil in
+          |> mspec σ.(genv_tu).(globals) (Tnamed cls) ty ti (Vptr $ _global dtor) (Vptr this :: nil) (fun _ => Q) in
+        match dtor with
+        | None =>
+          (*        |={↑pred_ns}=> this |-> tblockR t 1 ** (this |-> tblockR t 1 -* Q) *)
+          match σ.(genv_tu) !! cls with
+          | Some (Gstruct s) => continue s.(s_dtor)
+          | Some (Gunion u) => continue u.(u_dtor)
+          | _ => False
+          end
+        | Some dtor => continue dtor
+        end
     | Tarray t sz =>
       fold_right (fun i Q => valid_ptr (this .[ t ! Z.of_nat i ]) **
-         destruct_val t (this .[ t ! Z.of_nat i ]) dtor Q) Q (List.rev (seq 0 (N.to_nat sz)))
+         destruct_val dispatch t (this .[ t ! Z.of_nat i ]) dtor Q) Q (List.rev (seq 0 (N.to_nat sz)))
     | _ =>
-      (* |={↑pred_ns}=> *) this |-> anyR t 1 ** (this |-> tblockR t 1 -* Q)
+      (* |={↑pred_ns}=> *) this |-> anyR (erase_qualifiers t) 1 ** (this |-> tblockR (erase_qualifiers t) 1 -* Q)
       (* emp *)
-    end.
+    end%I.
+
+
+  Lemma destruct_val_frame dispatch : forall ty this dt Q Q',
+      Q -* Q' |-- destruct_val dispatch ty this dt Q -* destruct_val dispatch ty this dt Q'.
+  Proof.
+    induction ty; simpl; eauto;
+      try solve [
+            intros; iIntros "Q [$ X]"; iIntros "A"; iApply "Q"; iApply "X"; eauto ].
+    { induction (rev _); simpl; eauto.
+      intros.
+      iIntros "Q [$ V]"; iRevert "V"; iApply IHty; iApply IHl; eauto. }
+    { destruct dispatch.
+      { intros. iIntros "X"; iApply resolve_dtor_frame.
+        iIntros (???) "Y"; iNext; iRevert "Y".
+        iApply mspec_frame.
+        iIntros (?); eauto. }
+      { destruct dt.
+        - iIntros (??) "X Y"; iNext; iRevert "Y"; iApply mspec_frame; iIntros (?); eauto.
+        - case_match; eauto.
+        case_match; eauto.
+          + iIntros (??) "X Y"; iNext; iRevert "Y"; iApply mspec_frame; iIntros (?); eauto.
+          + iIntros (??) "X Y"; iNext; iRevert "Y"; iApply mspec_frame; iIntros (?); eauto. } }
+  Qed.
 
 End destroy.
