theories/lang/cpp/logic/expr.v
@@ -686,7 +686,7 @@ Module Type Expr.
       let raw_type := erase_qualifiers ty in
       Forall addr : ptr, addr |-> tblockR raw_type 1 -*
         wp_init ty addr e (fun free =>
-           Q (Vptr addr) (free ** destruct_val raw_type addr None (addr |-> tblockR raw_type 1))).
+           Q (Vptr addr) (free ** destruct_val false raw_type addr None (addr |-> tblockR raw_type 1))).
     (* XXX This use of [Vptr] represents an aggregate.
        XXX The destruction of the value isn't quite correct because we explicitly
            generate the destructors.
@@ -798,8 +798,8 @@ Module Type Expr.
       wp_glval vc obj (fun this free => wp_args es (fun vs free' =>
           match class_type (type_of obj) with
           | Some cls =>
-            resolve_virtual (σ:=resolve) this cls f (fun fimpl_addr thisp =>
-              |> mspec (type_of obj) (normalize_type fty) ti (Vptr fimpl_addr) (Vptr thisp :: vs) (fun v =>
+            resolve_virtual (σ:=resolve) this cls f (fun fimpl_addr impl_class thisp =>
+              |> mspec (Tnamed impl_class) (normalize_type fty) ti (Vptr fimpl_addr) (Vptr thisp :: vs) (fun v =>
                        Exists p, [| v = Vptr p |] ** Q p (free ** free')))
           | _ => False
           end))
@@ -809,8 +809,8 @@ Module Type Expr.
       wp_glval vc obj (fun this free => wp_args es (fun vs free' =>
           match class_type (type_of obj) with
           | Some cls =>
-            resolve_virtual (σ:=resolve) this cls f (fun fimpl_addr thisp =>
-              |> mspec (type_of obj) (normalize_type fty) ti (Vptr fimpl_addr) (Vptr thisp :: vs) (fun v =>
+            resolve_virtual (σ:=resolve) this cls f (fun fimpl_addr impl_type thisp =>
+              |> mspec (Tnamed impl_type) (normalize_type fty) ti (Vptr fimpl_addr) (Vptr thisp :: vs) (fun v =>
                        Exists p, [| v = Vptr p |] ** Q p (free ** free')))
           | _ => False
           end))
@@ -823,8 +823,8 @@ Module Type Expr.
            wp_glval vc obj (fun this free => wp_args es (fun vs free' =>
           match class_type (type_of obj) with
           | Some cls =>
-            resolve_virtual (σ:=resolve) this cls f (fun fimpl_addr thisp =>
-              |> mspec (type_of obj) (normalize_type fty) ti (Vptr fimpl_addr) (Vptr thisp :: vs) (fun v => Q v (free ** free')))
+            resolve_virtual (σ:=resolve) this cls f (fun fimpl_addr impl_class thisp =>
+              |> mspec (Tnamed impl_class) (normalize_type fty) ti (Vptr fimpl_addr) (Vptr thisp :: vs) (fun v => Q v (free ** free')))
          | _ => False
           end)))
       |-- wp_prval (Emember_call (inl (f, Virtual, fty)) vc obj es ty) Q.
@@ -836,8 +836,8 @@ Module Type Expr.
       wp_glval vc obj (fun this free => wp_args es (fun vs free' =>
           match class_type (type_of obj) with
           | Some cls =>
-            resolve_virtual (σ:=resolve) this cls f (fun fimpl_addr thisp =>
-              |> mspec (type_of obj) (normalize_type fty) ti (Vptr fimpl_addr) (Vptr thisp :: vs) (fun res => [| res = Vptr addr |] -* Q (free ** free')))
+            resolve_virtual (σ:=resolve) this cls f (fun fimpl_addr impl_class thisp =>
+              |> mspec (Tnamed impl_class) (normalize_type fty) ti (Vptr fimpl_addr) (Vptr thisp :: vs) (fun res => [| res = Vptr addr |] -* Q (free ** free')))
             (* NOTE as with other function calls, we are assuming an equation on the address in order
                to express the fact the the object is constructed in-place.
              *)
@@ -935,7 +935,7 @@ Module Type Expr.
           Exists obj_ptr storage_ptr sz,
             [| v = Vptr obj_ptr |] **
             [| size_of destroyed_type = Some sz |] **
-            destruct_val destroyed_type obj_ptr dtor   (* Calling destructor with object pointer *)
+            destruct_val true destroyed_type obj_ptr dtor   (* Calling destructor with object pointer *)
               (provides_storage storage_ptr obj_ptr ty ** (* Token for converting obj memory to storage memory *)
                obj_ptr |-> anyR destroyed_type 1 **    (* A trade; similar to end_provides_storage. *)
                 (storage_ptr |-> blockR sz 1 -*
@@ -961,7 +961,7 @@ Module Type Expr.
          Forall a : ptr, a |-> tblockR raw_type 1 -*
                   let '(e,dt) := destructor_for e in
                   wp_init ty a e
-                          (fun free => Q a (destruct_val ty a dt (a |-> tblockR raw_type 1 ** free))))
+                          (fun free => Q a (destruct_val false ty a dt (a |-> tblockR raw_type 1 ** free))))
         |-- wp_xval (Ematerialize_temp e ty) Q.
 
     (** temporary materialization only occurs when the resulting value is used.
@@ -979,7 +979,7 @@ Module Type Expr.
          Forall a : ptr, a |-> tblockR raw_type 1 -*
                    let '(e,dt) := destructor_for e in
                    wp_init ty a e (fun free =>
-                                     Q (Vptr a) (destruct_val ty a dt (a |-> tblockR raw_type 1 ** free))))
+                                     Q (Vptr a) (destruct_val false ty a dt (a |-> tblockR raw_type 1 ** free))))
         |-- wp_prval e Q.
 
 
@@ -1004,7 +1004,7 @@ Module Type Expr.
       let raw_type := erase_qualifiers ty in
       a |-> tblockR raw_type 1 -*
           wp_init ty a e (fun free =>
-                            Q (Vptr a) (destruct_val ty a (Some dtor) (a |-> tblockR raw_type 1 ** free))))
+                            Q (Vptr a) (destruct_val false ty a (Some dtor) (a |-> tblockR raw_type 1 ** free))))
       |-- wp_prval (Ebind_temp e dtor ty) Q.
 
     (** Pseudo destructors arise from calling the destructor on
